finally got a class invariant for blood inventory

Dafny/BloodInventory.dfy
@@ -2,49 +2,30 @@ include "Blood.dfy"
 class BloodInventory
 {
     var bloodInventory: array<Blood>;
+    ghost var shadowBloodInventory: array<string>;
     var threshold: int;
     var alert: bool;
 
     predicate Valid()
-    requires bloodInventory != null
-    reads this, this.bloodInventory, set i | 0 <= i < bloodInventory.Length :: bloodInventory[i] 
-
+    requires shadowBloodInventory != null
+    reads this, this.shadowBloodInventory
     {
-        alert ==> (threshold >= CountByBloodType("A+")) 
+        forall i :: 0 <= i < shadowBloodInventory.Length ==> validBloodType(shadowBloodInventory[i]) && 
+        alert ==> (threshold >= multiset(shadowBloodInventory[..])["A+"]) &&
+        alert ==> (threshold >= multiset(shadowBloodInventory[..])["A-"]) &&
+        alert ==> (threshold >= multiset(shadowBloodInventory[..])["B+"]) &&
+        alert ==> (threshold >= multiset(shadowBloodInventory[..])["B-"]) &&
+        alert ==> (threshold >= multiset(shadowBloodInventory[..])["O+"]) &&
+        alert ==> (threshold >= multiset(shadowBloodInventory[..])["O-"]) &&
+        alert ==> (threshold >= multiset(shadowBloodInventory[..])["AB+"]) &&
+        alert ==> (threshold >= multiset(shadowBloodInventory[..])["AB-"])
     } 
 
-    function CountByBloodType(bloodType:string): int
-    requires bloodInventory != null
-    reads this, this.bloodInventory, set i | 0 <= i < bloodInventory.Length :: bloodInventory[i] 
-    // ensures CountByBloodType(bloodType) == CheckIndexForBloodType(bloodType,  bloodInventory.Length - 1)
-    {
-        CheckIndexForBloodType(bloodType,  bloodInventory.Length - 1)
-    }
-
-    function CheckIndexForBloodType(bloodType: string, index: int): int
-    requires bloodInventory != null
-    requires 0 <= index < bloodInventory.Length
-    requires bloodInventory[index] != null
-    requires (bloodInventory[index].GetBloodType() == "A+" || bloodInventory[index].GetBloodType() == "A-" || bloodInventory[index].GetBloodType() == "B+" || bloodInventory[index].GetBloodType() == "B-" ||
-              bloodInventory[index].GetBloodType() == "O+" || bloodInventory[index].GetBloodType() == "O-" || bloodInventory[index].GetBloodType() == "AB+" || bloodInventory[index].GetBloodType() == "AB-")
-    reads this, this.bloodInventory, set i | 0 <= i < bloodInventory.Length :: bloodInventory[i] 
-    decreases index
-    // ensures (index < 0) ==> (CheckIndexForBloodType(bloodType, index) == 0)
-    // ensures (index >= 0 && (bloodInventory[index].GetBloodType() == bloodType)) ==> (CheckIndexForBloodType(bloodType, index) == CheckIndexForBloodType(bloodType, index - 1) + 1) 
-    // ensures (index >= 0 && (bloodInventory[index].GetBloodType() != bloodType)) ==> (CheckIndexForBloodType(bloodType, index) == CheckIndexForBloodType(bloodType, index - 1)) 
-    {
-        if index == 0 
-        then
-            if bloodInventory[index].GetBloodType() == bloodType
-            then
-                1
-            else
-                0
-        else
-            if bloodInventory[index].GetBloodType() == bloodType
-            then
-                CheckIndexForBloodType(bloodType, index - 1) + 1
-            else
-                CheckIndexForBloodType(bloodType, index - 1)
-    }
 } // end of BloodInventory class
+
+predicate validBloodType(bloodType: string)
+{
+        bloodType == "A+" || bloodType == "A-" || bloodType == "B+" || bloodType == "B-" ||
+        bloodType == "O+" || bloodType == "O-" || bloodType == "AB+" || bloodType == "AB-"
+
+}
